@prefix : <http://www.semanticweb.org/owl/owlapi/turtle#> .
@prefix owl: <http://www.w3.org/2002/07/owl#> .
@prefix rdf: <http://www.w3.org/1999/02/22-rdf-syntax-ns#> .
@prefix xml: <http://www.w3.org/XML/1998/namespace> .
@prefix xsd: <http://www.w3.org/2001/XMLSchema#> .
@prefix rdfs: <http://www.w3.org/2000/01/rdf-schema#> .
@prefix ddhub: <http://ddhub.no/> .
@base <http://www.semanticweb.org/owl/owlapi/turtle#> .
@prefix zzz: <http://ddhub.demo/zzz#> .

###  http://ddhub.demo/zzz#commonlyUsedMnemonics
zzz:commonMnemonics rdf:type owl:AnnotationProperty ;
                            rdfs:range xsd:string .

###  http://ddhub.no/ThousandKilogramForce
ddhub:ThousandKilogramForce rdf:type owl:Class ;
                            rdfs:subClassOf ddhub:Unit ,
                                            [ rdf:type owl:Restriction ;
                                              owl:onProperty ddhub:IsUnitForQuantity ;
                                              owl:allValuesFrom [ a owl:Class ;
                                                        owl:unionOf ( ddhub:ForceQuantity ) ]
                                            ] ;
                            zzz:commonMnemonics "kkgf"@en ;
                            rdfs:comment "1 ThousandKilogramForce = 1000 KilogramForce." .

###  http://ddhub.no/ElectricPotentialQuantity
ddhub:ElectricPotentialQuantity a owl:Class ;
    rdfs:comment """The electric potential energy per unit charge. This value can be calculated in either a static (time-invariant) or a dynamic (time-varying) electric field at a specific time with the unit joules per coulomb (J⋅C−1) or volt (V).
"""@EN ;
    rdfs:subClassOf ddhub:Quantity .

###  http://ddhub.no/ConcentrationQuantity
ddhub:ConcentrationQuantity a owl:Class ;
    rdfs:comment """Concentration is the abundance of a constituent divided by the total volume of a mixture. Several types of mathematical description can be distinguished: mass concentration, molar concentration, number concentration, and volume concentration.
"""@EN ;
    rdfs:subClassOf ddhub:Quantity .

###  http://ddhub.no/ConcentrationQuantity
ddhub:ConcentrationGasDrillingQuantity a owl:Class ;
    rdfs:comment """For gas, the molar concentration or volume concentration are commonly used.
"""@EN ;
    rdfs:subClassOf ddhub:MeasurableQuantity .
